ProjProbVF.v
@@ -12,7 +12,7 @@ Open Scope Z.
 Inductive Op : Type :=
   | P   : Op
   | M   : Op
-  | MM   : Op.
+  | MM  : Op.
 
 
 Inductive aexp :=
@@ -48,6 +48,7 @@ Eval compute in aeval (([2];*;[3]);+;([3];*;([4];-;[2]))).
 Eval compute in (20-40)*(30+(1*1)).
 
 Eval compute in aeval (([20];-;[40]);*;([30];+;([1];*;[1]))).
+
 (*4*)
 
 Inductive Exp : Type :=
@@ -58,26 +59,26 @@ Inductive Exp : Type :=
   | LP    : Exp
   | RP    : Exp.
 
-(* Module ListNotations. *)
-(* Notation "[ ]" := nil (format "[ ]") : list_scope. *)
-(* Notation "[ x ]" := (cons x nil) : list_scope. *)
-(* Notation "[ x ; y ; .. ; z ]" := (cons x (cons y .. (cons z nil) ..)) : list_scope. *)
-(* End ListNotations. *)
-(*  *)
-(* Import ListNotations. *)
-(*  *)
-(* Fixpoint abc (a : aexp) : list Exp := *)
-(*    match a with *)
-(*     | Node L P R  => [LP] ++ abc L ++ [RP] ++ [Pls] ++ [LP] ++ abc R ++ [RP]  *)
-(*     | Node L M R  => [LP] ++ abc L ++ [RP] ++ [Min] ++ [LP] ++ abc R ++ [RP]   *)
-(*     | Node L MM R => [LP] ++ abc L ++ [RP] ++ [Mul] ++ [LP] ++ abc R ++ [RP]  *)
-(*     | Leaf n => [Num n]  *)
-(* end. *)
-(* Eval compute in abc ([2];*;[3]). *)
-(*  *)
-(* Eval compute in abc (([2];*;[3]);+;([3];*;([4];-;[2]))). *)
+Module ListNotations.
+Notation "[ ]" := nil (format "[ ]") : list_scope.
+Notation "[ x ]" := (cons x nil) : list_scope.
+Notation "[ x ; y ; .. ; z ]" := (cons x (cons y .. (cons z nil) ..)) : list_scope.
+End ListNotations.
 
-(* isto é equivalente a : ((2) * (3)) + ((3) *((4)-(2))) *) 
+Import ListNotations.
+
+Fixpoint abc (a : aexp) : list Exp :=
+   match a with
+    | Node L P R  => [LP] ++ abc L ++ [RP] ++ [Pls] ++ [LP] ++ abc R ++ [RP] 
+    | Node L M R  => [LP] ++ abc L ++ [RP] ++ [Min] ++ [LP] ++ abc R ++ [RP]  
+    | Node L MM R => [LP] ++ abc L ++ [RP] ++ [Mul] ++ [LP] ++ abc R ++ [RP] 
+    | Leaf n => [Num n] 
+end.
+Eval compute in abc ([2];*;[3]).
+
+Eval compute in abc (([2];*;[3]);+;([3];*;([4];-;[2])))
+
+isto é equivalente a : ((2) * (3)) + ((3) *((4)-(2)))
 
 Eval compute in ((2) * (3)) + ((3) *((4)-(2))).
 
@@ -100,44 +101,67 @@ Theorem RelEqFun : forall (a : aexp) (n : Z),
                     (aevalR a n) <-> (aeval a = n).
 Proof.
   induction a.
-  - red.
-     
+  - simpl. intros. reflexivity.
+  - red. intros. induction o.
+    + split.
+        simpl. intros. 
+        destruct H as [n1 H]. 
+        destruct H as [n2 H]. 
+        destruct H. destruct H0. 
+        assert (IHa1 := (IHa1 n1)).
+        assert (IHa2 := (IHa2 n2)).
+        unfold iff in IHa1; destruct IHa1; clear H3.
+        unfold iff in IHa2; destruct IHa2; clear H4.
+        assert (H5 := (H2 H)).
+        assert (H6 := (H3 H0)).
+        rewrite H5; rewrite H6.
+        assumption.
+      * simpl. intros.
+        assert (IHa1 := (IHa1 (aeval a1))).
+        assert (IHa2 := (IHa2 (aeval a2))).
+        unfold iff in IHa1; destruct IHa1; clear H0.
+        unfold iff in IHa2. destruct IHa2. clear H0.
+        exists (aeval a1); exists (aeval a2).
+        auto.
+    + split.
+      * simpl. intros. 
+        destruct H as [n1 H]. 
+        destruct H as [n2 H]. 
+        destruct H. destruct H0. 
+        assert (IHa1 := (IHa1 n1)).
+        assert (IHa2 := (IHa2 n2)).
+        unfold iff in IHa1; destruct IHa1; clear H3.
+        unfold iff in IHa2; destruct IHa2; clear H4.
+        assert (H5 := (H2 H)).
+        assert (H6 := (H3 H0)).
+        rewrite H5; rewrite H6.
+        assumption.
+      * simpl. intros.
+        assert (IHa1 := (IHa1 (aeval a1))).
+        assert (IHa2 := (IHa2 (aeval a2))).
+        unfold iff in IHa1; destruct IHa1; clear H0.
+        unfold iff in IHa2. destruct IHa2. clear H0.
+        exists (aeval a1); exists (aeval a2).
+        auto.
+    + split.
+      * simpl. intros. 
+        destruct H as [n1 H]. 
+        destruct H as [n2 H]. 
+        destruct H. destruct H0. 
+        assert (IHa1 := (IHa1 n1)).
+        assert (IHa2 := (IHa2 n2)).
+        unfold iff in IHa1; destruct IHa1; clear H3.
+        unfold iff in IHa2; destruct IHa2; clear H4.
+        assert (H5 := (H2 H)).
+        assert (H6 := (H3 H0)).
+        rewrite H5; rewrite H6.
+        assumption.
+      * simpl. intros.
+        assert (IHa1 := (IHa1 (aeval a1))).
+        assert (IHa2 := (IHa2 (aeval a2))).
+        unfold iff in IHa1; destruct IHa1; clear H0.
+        unfold iff in IHa2. destruct IHa2. clear H0.
+        exists (aeval a1); exists (aeval a2).
+        auto.
 Qed.
-(*
-Proof.
-  intros.
-  red.
-  split.
-  - induction a.
-    + simpl; intros; assumption.
-    + induction o.
-      * simpl; intros.
-        exists (aeval a1).
-      * simpl; intros; admit.
-      * simpl; intros; admit.
-  - induction a.
-    + simpl; intros; assumption.
-    + induction o.
-      * simpl; intros.
-        exists (aeval a1);exists (aeval a2).
-        split.
-        -- let n:=(aeval a1) in IHa1.
-        -- split.
-           ++ admit.
-           ++ assumption.
-      * simpl; intros; admit.
-      * simpl; intros; admit.
-Qed.
-*)
-(* for th simple case where aevalR a n = (aeval a = n)
-Proof.
-  induction a.
-    - intros.
-      red.
-      simpl.
-      split;[intros; assumption | intros; assumption].
-    - intros.
-      red.
-      split;[simpl; intros;assumption| simpl; intros;assumption].
-Qed.
-*)
+
